backend/ValueDomain.v
@@ -3438,7 +3438,7 @@ Lemma ablock_init_sound:
   forall m b p, smatch m b p -> bmatch m b (ablock_init p).
 Proof.
   intros; split; auto; intros.
-  unfold ablock_load, ablock_init; simpl. rewrite ZTree.gempty.
+  unfold ablock_load, ablock_init; simpl.
   eapply vnormalize_cast; eauto. eapply H; eauto.
 Qed.
 
@@ -4558,7 +4558,7 @@ Lemma ematch_init:
   ematch (init_regs vl rl) (einit_regs rl).
 Proof.
   induction rl; simpl; intros.
-- red; intros. rewrite Regmap.gi. simpl AE.get. rewrite PTree.gempty.
+- red; intros. rewrite Regmap.gi. simpl.
   constructor.
 - destruct vl as [ | v1 vs ].
   + assert (ematch (init_regs nil rl) (einit_regs rl)).
