cfrontend/Cminorgenproof.v
@@ -875,7 +875,6 @@ Proof.
   intros. apply Mem.perm_implies with Freeable; auto with mem. eapply Mem.perm_alloc_2; eauto.
   instantiate (1 := f1). red; intros. eelim Mem.fresh_block_alloc; eauto.
   eapply Mem.valid_block_inject_2; eauto.
-  intros. apply PTree.gempty.
   eapply match_callstack_alloc_right; eauto.
   intros. destruct (In_dec peq id (map fst vars)).
   apply cenv_remove_gss; auto.
