common/Memory.v
@@ -346,15 +346,6 @@ Program Definition empty: mem :=
   mkmem (PMap.init (ZMap.init Undef))
         (PMap.init (fun ofs k => None))
         1%positive _ _ _.
-Next Obligation.
-  repeat rewrite PMap.gi. red; auto.
-Qed.
-Next Obligation.
-  rewrite PMap.gi. auto.
-Qed.
-Next Obligation.
-  rewrite PMap.gi. auto.
-Qed.
 
 (** Allocation of a fresh block with the given bounds.  Return an updated
   memory state and the address of the fresh block, which initially contains
@@ -631,7 +622,7 @@ Proof. reflexivity. Qed.
 
 Theorem perm_empty: forall b ofs k p, ~perm empty b ofs k p.
 Proof.
-  intros. unfold perm, empty; simpl. rewrite PMap.gi. simpl. tauto.
+  intros. unfold perm, empty; simpl. tauto.
 Qed.
 
 Theorem valid_access_empty: forall chunk b ofs p, ~valid_access empty chunk b ofs p.
